\item \$y=\textbackslash frac\{2\}\{\{\{x\}\textasciicircum\{2\}\}-3\}\textbackslash xrightarrow\{A\}y=\textbackslash frac\{2\}\{\{\{(x+a)\}\textasciicircum\{2\}\}-3\}\textbackslash xrightarrow\{B\}y=\textbackslash frac\{2\}\{\{\{(-x+a)\}\textasciicircum\{2\}\}-3\}\$
\$\textbackslash xrightarrow\{C\}\textbackslash frac\{y\}\{b\}=\textbackslash frac\{2\}\{\{\{(-x+a)\}\textasciicircum\{2\}\}-3\}\textbackslash Rightarrow
y=\textbackslash frac\{2b\}\{\{\{x\}\textasciicircum\{2\}\}-2ax+\{\{a\}\textasciicircum\{2\}\}-3\}\$
Comparing with\$y=\textbackslash frac\{6\}\{\{\{x\}\textasciicircum\{2\}\}-10x+22\},\$
\$\textbackslash begin\{align\} \& -2a=-10\textbackslash Rightarrow
a=5 \textbackslash\textbackslash{} \& b=3 \textbackslash\textbackslash{}
\textbackslash end\{align\}\$

Alternatively, \$y=\textbackslash frac\{6\}\{\{\{x\}\textasciicircum\{2\}\}-10x+22\}=\textbackslash frac\{6\}\{\{\{(5-x)\}\textasciicircum\{2\}\}-3\}\textbackslash Rightarrow
\textbackslash frac\{y\}\{3\}=\textbackslash frac\{2\}\{\{\{(5-x)\}\textasciicircum\{2\}\}-3\}\$
\$\textbackslash therefore a=5,\textbackslash text\{ \}b=3\$