\item {}

(i) For \$\{\{C\}\_\{2\}\},\$ when \textbackslash{[}x=0,\textbackslash{]}

\textbackslash{[}\textbackslash begin\{align\} \& 2\{\{\textbackslash text\{e\}\}\textasciicircum\{-t\}\}-4\{\{\textbackslash text\{e\}\}\textasciicircum\{2t\}\}=0
\textbackslash\textbackslash{} \& 4\{\{\textbackslash text\{e\}\}\textasciicircum\{2t\}\}=2\{\{\textbackslash text\{e\}\}\textasciicircum\{-t\}\}
\textbackslash\textbackslash{} \& \{\{\textbackslash text\{e\}\}\textasciicircum\{3t\}\}=\textbackslash frac\{1\}\{2\}
\textbackslash\textbackslash{} \& t=\textbackslash frac\{1\}\{3\}\textbackslash ln
\textbackslash frac\{1\}\{2\}=-\textbackslash frac\{1\}\{3\}\textbackslash ln
2 \textbackslash end\{align\}\textbackslash{]}

Therefore,

\textbackslash{[}y=3\{\{\textbackslash text\{e\}\}\textasciicircum\{\textbackslash frac\{1\}\{3\}\textbackslash ln
2\}\}+\{\{\textbackslash text\{e\}\}\textasciicircum\{-\textbackslash frac\{2\}\{3\}\textbackslash ln
2\}\}=4.41\textbackslash text\{ (to 3 s\}\textbackslash text\{.f\}\textbackslash text\{.)\}\textbackslash{]}

(ii) \textbackslash{[}x=2\{\{\textbackslash text\{e\}\}\textasciicircum\{-t\}\}-4\{\{\textbackslash text\{e\}\}\textasciicircum\{2t\}\}(1)\textbackslash{]}
\textbackslash{[}y=3\{\{\textbackslash text\{e\}\}\textasciicircum\{-t\}\}+\{\{\textbackslash text\{e\}\}\textasciicircum\{2t\}\}(2)\textbackslash{]}
\$2\textbackslash times (2)-3\textbackslash times (1):2y-3x=14\{\{\textbackslash text\{e\}\}\textasciicircum\{2t\}\}(3)\$
\$\textbackslash begin\{align\} \& 4\textbackslash times (2)+1\textbackslash times
(1):4y+x=14\{\{\textbackslash text\{e\}\}\textasciicircum\{-t\}\}
\textbackslash\textbackslash{} \& \{\{\textbackslash text\{e\}\}\textasciicircum\{t\}\}=\textbackslash frac\{14\}\{x+4y\}(4)
\textbackslash\textbackslash{} \textbackslash end\{align\}\$ Substituting
(4) into (3), \$2y-3x=14\{\{\textbackslash left( \textbackslash frac\{14\}\{x+4y\}
\textbackslash right)\}\textasciicircum\{2\}\}\$ \$\{\{\textbackslash left(
x+4y \textbackslash right)\}\textasciicircum\{2\}\}\textbackslash left(
2y-3x \textbackslash right)=2744\$