\item {}
\begin{enumerate}
\item[(i)]  $\overrightarrow{OA}=\left(\begin{matrix}4\\
-2\\
0
\end{matrix}\right)\overrightarrow{OB}=\left(\begin{matrix}\alpha\\
-1\\
2
\end{matrix}\right)\overrightarrow{OC}=\left(\begin{matrix}-1\\
-7\\
\beta
\end{matrix}\right)$

$A$, $B$ and $C$ are collinear.

$\therefore\overrightarrow{AB}=k\overrightarrow{AC}$

$\left(\begin{matrix}\alpha-4\\
1\\
2
\end{matrix}\right)=k\left(\begin{matrix}-5\\
-5\\
\beta
\end{matrix}\right)\Rightarrow\left\{ \begin{matrix}\alpha-4=-5k\\
1=-5k\\
2=k\beta
\end{matrix}\right.\Rightarrow\left\{ \begin{matrix}k=-\frac{1}{5}\\
\alpha=5\\
\beta=-10
\end{matrix}\right.$
\item[(ii)]  $\overrightarrow{OP}=\left(\begin{matrix}2\\
3\\
0
\end{matrix}\right)$ is position vector of a point on the line $L$. 

$\overrightarrow{AP}=\left(\begin{matrix}2\\
3\\
0
\end{matrix}\right)-\left(\begin{matrix}4\\
-2\\
0
\end{matrix}\right)=\left(\begin{matrix}-2\\
5\\
0
\end{matrix}\right)$ 

Distance from $A$ to $L$ = 

\begin{align*}
 & \left|\overrightarrow{AP}\times\frac{1}{\sqrt{4+1+1}}\left(\begin{matrix}2\\
-1\\
1
\end{matrix}\right)\right|\\
= & \frac{1}{\sqrt{6}}\left|\left(\begin{matrix}-2\\
5\\
0
\end{matrix}\right)\times\left(\begin{matrix}2\\
-1\\
1
\end{matrix}\right)\right|\\
= & \frac{1}{\sqrt{6}}\left|\left(\begin{matrix}5\\
2\\
-8
\end{matrix}\right)\right|\\
= & \frac{1}{\sqrt{6}}\sqrt{25+4+64}\\
= & \sqrt{\frac{93}{6}}\\
= & \sqrt{\frac{31}{2}}.
\end{align*}

\item[(iii)]  Normal of plane $\pi=\overrightarrow{AB}\times\left(\begin{matrix}2\\
-1\\
1
\end{matrix}\right)=\left(\begin{matrix}1\\
1\\
2
\end{matrix}\right)\times\left(\begin{matrix}2\\
-1\\
1
\end{matrix}\right)=\left(\begin{matrix}3\\
3\\
-3
\end{matrix}\right)=3\left(\begin{matrix}1\\
1\\
-1
\end{matrix}\right)$

Equation of plane $\pi\text{: }\mathbf{r}\cdot\left(\begin{matrix}1\\
1\\
-1
\end{matrix}\right)=\left(\begin{matrix}2\\
3\\
0
\end{matrix}\right)\centerdot\left(\begin{matrix}1\\
1\\
-1
\end{matrix}\right)=2+3=5$

Cartesian equation is $x+y-z=5$
\item[(iv)]  Let $F$ be the foot of perpendicular from $A(4,-2,0)$ to the plane
$\pi$

Equation of line $AF$: $\mathbf{r}=\left(\begin{matrix}4\\
-2\\
0
\end{matrix}\right)+\lambda\left(\begin{matrix}1\\
1\\
-1
\end{matrix}\right)=\left(\begin{matrix}4+\lambda\\
-2+\lambda\\
-\lambda
\end{matrix}\right)$ 

To find the point of intersection of line $AF$ and plane $\pi$,
substitute equation of line into equation of plane $x+y-z=5$. 

$\begin{array}{ccc}
 & 4+\lambda-2+\lambda+\lambda & =5\\
\Rightarrow & 3\lambda+2 & =5\\
\Rightarrow & \lambda & =1
\end{array}$

$\therefore\overrightarrow{OF}=\left(\begin{matrix}4\\
-2\\
0
\end{matrix}\right)+1\left(\begin{matrix}1\\
1\\
-1
\end{matrix}\right)=\left(\begin{matrix}5\\
-1\\
-1
\end{matrix}\right)$

\textbf{Alternative method }

$\overrightarrow{OD}=\left(\begin{matrix}2\\
3\\
0
\end{matrix}\right)$ is a point on the plane $\pi$. $\overrightarrow{DA}=\left(\begin{matrix}2\\
-5\\
0
\end{matrix}\right)$ 

$\overrightarrow{FA}=$ Projected vector of $\overrightarrow{DA}$
on normal of plane. 

$\begin{array}{ccc}
\overrightarrow{FA} & =\left(\overrightarrow{DA}\cdot\mathbf{\hat{n}}\right)\mathbf{\hat{n}} & \text{where }\mathbf{n}\text{ is the normal of }ABC\\
 & =\frac{\left(\left(\begin{matrix}2\\
-5\\
0
\end{matrix}\right)\cdot\left(\begin{matrix}1\\
1\\
-1
\end{matrix}\right)\right)\left(\begin{matrix}1\\
1\\
-1
\end{matrix}\right)}{\sqrt{1+1+1}\sqrt{1+1+1}}\\
 & =\frac{2-5}{3}\left(\begin{matrix}1\\
1\\
-1
\end{matrix}\right)=-\left(\begin{matrix}1\\
1\\
-1
\end{matrix}\right)=\left(\begin{matrix}-1\\
-1\\
1
\end{matrix}\right)
\end{array}$

$\therefore\overrightarrow{OF}=\overrightarrow{OA}-\overrightarrow{FA}=\left(\begin{matrix}4\\
-2\\
0
\end{matrix}\right)-\left(\begin{matrix}-1\\
-1\\
1
\end{matrix}\right)=\left(\begin{matrix}5\\
-1\\
-1
\end{matrix}\right)$ 

Let the reflection of $A$ about plane $\pi$ be $A\lyxmathsym{\textquoteright}(x,y,z)$ 

\begin{align*}
\overrightarrow{AF} & =\overrightarrow{FA'}\\
\overrightarrow{OA'} & =2\overrightarrow{OF}-\overrightarrow{OA}\\
\overrightarrow{OA'} & =2\left(\begin{matrix}5\\
-1\\
-1
\end{matrix}\right)-\left(\begin{matrix}4\\
-2\\
0
\end{matrix}\right)=\left(\begin{matrix}6\\
0\\
-2
\end{matrix}\right)
\end{align*}
 

Alternatively:

\begin{align*}
\frac{4+x}{2} & =5 & \implies x=6\\
\frac{-2+y}{2} & =-1 & \implies y=0\\
\frac{0+z}{2} & =-1 & \implies z=-2
\end{align*}

Equation of reflected line is: 

$\mathbf{r}=\left(\begin{matrix}6\\
0\\
-2
\end{matrix}\right)+\lambda\left(\begin{matrix}1\\
1\\
2
\end{matrix}\right)$
\end{enumerate}