\item {}
\begin{enumerate}
\item[(a)]  

\begin{align*}
 & \sum\limits _{r=7}^{n+1}\left(2^{r}+r^{2}-r\right)\\
= & \sum\limits _{r=7}^{n+1}\left(2^{r}\right)+\sum\limits _{r=7}^{n+1}\left(r^{2}\right)-\sum\limits _{r=7}^{n+1}\left(r\right)\\
= & \frac{2^{7}\left(2^{n-5}-1\right)}{2-1}+\sum\limits _{r=1}^{n+1}\left(r^{2}\right)-\sum\limits _{r=1}^{6}\left(r^{2}\right)-\left(\frac{n-5}{2}\right)\left(7+n+1\right)\\
= & 2^{7}\left(2^{n-5}-1\right)+\frac{\left(n+1\right)}{6}\left(n+2\right)\left(2n+3\right)-\left(\frac{6}{6}\right)\left(7\right)\left(13\right)-\left(\frac{n-5}{2}\right)\left(8+n\right)\\
= & 2^{7}\left(2^{n-5}-1\right)+\frac{\left(n+1\right)}{6}\left(n+2\right)\left(2n+3\right)-91-\frac{\left(n-5\right)\left(8+n\right)}{2}
\end{align*}

Alternative Method: 
\begin{align*}
 & \sum\limits _{r=7}^{n+1}\left(2^{r}+r^{2}-r\right)\\
= & \sum\limits _{r=1}^{n+1}\left(2^{r}+r^{2}-r\right)-\sum\limits _{r=1}^{6}\left(2^{r}+r^{2}-r\right)\\
= & \frac{2\left(2^{n+1}-1\right)}{2-1}+\frac{1}{6}\left(n+1\right)\left(n+2\right)\left(2n+3\right)-\frac{n+1}{2}\left(1+n+1\right)\\
= & \frac{2\left(2^{6}-1\right)}{2-1}-91+\frac{6}{2}\left(1+6\right)\\
= & 2^{n+2}+\frac{1}{6}\left(n+1\right)\left(n+2\right)\left(2n+3\right)-\frac{\left(n+1\right)\left(n+2\right)}{2}-198\\
= & 2^{n+2}+\left[\frac{\left(n+1\right)\left(n+2\right)}{6}\right]\left(2n+3-3\right)-198\\
= & 2^{n+2}+\frac{1}{3}n\left(n+1\right)\left(n+2\right)-198
\end{align*}

\item[(a)]  
\begin{enumerate}
\item[(i)]  Using partial fractions,

\begin{align*}
\frac{1}{r^{2}-1} & =\frac{1}{2}\left(\frac{1}{r-1}-\frac{1}{r+1}\right)\\
\sum\limits _{r=2}^{n}\frac{1}{r^{2}-1} & =\frac{1}{2}\sum\limits _{r=2}^{n}\left(\frac{1}{r-1}-\frac{1}{r+1}\right)\\
 & =\frac{1}{2}\left[\begin{array}{cccc}
 & \frac{1}{1} & - & \frac{1}{3}\\
+ & \frac{1}{2} & - & \frac{1}{4}\\
+ & \frac{1}{3} & - & \frac{1}{5}\\
 & \vdots\\
+ & \frac{1}{n-3} & - & \frac{1}{n-1}\\
+ & \frac{1}{n-2} & - & \frac{1}{n}\\
+ & \frac{1}{n-1} & - & \frac{1}{n+1}
\end{array}\right]\\
 & =\frac{1}{2}\left(\frac{3}{2}-\frac{1}{n}-\frac{1}{n+1}\right)\\
 & =\frac{3}{4}+\frac{-\frac{1}{2}}{n}+\frac{-\frac{1}{2}}{n+1}
\end{align*}
 

$\therefore A=-\frac{1}{2}$. 
\item[(ii) ] As $n\to\infty$, $\frac{1}{n}\to0$, $\frac{1}{n+1}\to0$, therefore
$\sum\limits _{r=2}^{\infty}\frac{1}{r^{2}-1}$ converges. $\sum\limits _{r=2}^{\infty}\frac{1}{r^{2}-1}=\frac{3}{4}$. 
\item[(iii)]  $\frac{2}{2^{2}}+\frac{2}{3^{2}}+\frac{2}{4^{2}}+...=\sum\limits _{r=2}^{\infty}\frac{2}{r^{2}}$

Since $r^{2}-1<r^{2}$,

$\therefore$. 

\begin{align*}
\frac{2}{r^{2}-1} & >\frac{2}{r^{2}}\\
\sum\limits _{r=2}^{\infty}\frac{2}{r^{2}-1} & >\sum\limits _{r=2}^{\infty}\frac{2}{r^{2}}\\
\sum\limits _{r=2}^{\infty}\frac{2}{r^{2}} & <2\left(\frac{3}{4}\right)\\
\frac{2}{2^{2}}+\frac{2}{3^{2}}+\frac{2}{4^{2}}+.. & <\frac{3}{2} & (\text{shown})
\end{align*}

\end{enumerate}
\end{enumerate}