\item {}
\begin{enumerate}
\item[(i)]  Using Ratio Theorem $\overrightarrow{OC}=\frac{1}{k+1}(\mathbf{a}+k\mathbf{b})$ 
\item[(ii)]  Length of projection of $\overrightarrow{OC}$ onto$\overrightarrow{OA}$
= 

\begin{align*}
\frac{\left|\overrightarrow{OC}\cdot\mathbf{a}\right|}{\left|\mathbf{a}\right|} & =\frac{\left|\frac{1}{k+1}(\mathbf{a}+k\mathbf{b})\cdot\mathbf{a}\right|}{2}\\
 & =\frac{1}{2\left(k+1\right)}\left|(\mathbf{a}+k\mathbf{b})\cdot\mathbf{a}\right| & \text{since }0<k<1\\
 & =\frac{1}{2\left(k+1\right)}\left|(\mathbf{a}\cdot\mathbf{a}+k\mathbf{b}\cdot\mathbf{a})\right|\\
 & =\frac{1}{2\left(k+1\right)}\left|\left|\mathbf{a}\right|^{2}+k\mathbf{b}\cdot\mathbf{a}\right|\\
 & \,=\frac{1}{2\left(k+1\right)}\left|4+k\left|\mathbf{a}\right|\left|\mathbf{b}\right|\cos\left(60^{\circ}\right)\right|\\
 & =\frac{1}{2\left(k+1\right)}\left|4+k\left(2\right)\left(1\right)\left(\frac{1}{2}\right)\right|\\
 & =\frac{4+k}{2\left(k+1\right)} & \text{(proved)}
\end{align*}

\item[(iii)]  Area of triangle OAC =
\begin{align*}
\frac{1}{2}\left|\mathbf{a}\times\text{\ensuremath{\mathbf{c}}}\right| & =\frac{1}{2}\left|\mathbf{a}\times\frac{1}{k+1}\left(\mathbf{a}+k\left|\mathbf{b}\right|\right)\right|\\
 & =\frac{1}{2(k+1)}\left|(\mathbf{a}\times\mathbf{a})+k(\mathbf{a}\times\left|\mathbf{b}\right|)\right| & \text{since }0<k<1\\
 & =\frac{1}{2(k+1)}\left|(k(\mathbf{a}\times\left|\mathbf{b}\right|)\right| & \text{since}(\mathbf{a}\times\mathbf{a})=\mathbf{0}\\
 & =\frac{k}{2(k+1)}\left|\left|\mathbf{a}\right|\left|\mathbf{b}\right|\sin\left(60^{\circ}\right)\right|\\
 & =\frac{k}{2(k+1)}\left|2(1)\frac{\sqrt{3}}{2}\right|\\
 & =\frac{\sqrt{3}k}{2(k+1)}
\end{align*}
\end{enumerate}