\item {}
\begin{enumerate}
\item[(i)]  
\noindent \begin{center}
<INSERT\_IMAGE\_HERE>
\par\end{center}
\item[(ii)]  $y=\frac{1}{\left|1-x^{2}\right|}=\pm\frac{1}{1-x^{2}}$. 

Considering the interval $-2\le x<-1$, 

\begin{align*}
y & =-\frac{1}{1-x^{2}}\\
y & =\frac{1}{x^{2}-1}\\
yx^{2}-y & =1\\
x^{2} & =\frac{1+y}{y}\\
x & =\pm\sqrt{\frac{1+y}{y}}\\
x & =-\sqrt{\frac{1+y}{y}} & (\text{since}-2\le x<-1)\\
\text{f}^{-1}(x) & =-\sqrt{\frac{1+x}{x}}\\
 & =-\sqrt{\frac{1}{x}+1}
\end{align*}

$\text{D}_{\text{f}^{-1}}=\text{R}_{\text{f}}=[\frac{1}{3},\infty)$
\item[(iii)]  Since $R_{\text{f}}=[\tfrac{1}{3},\infty)\subseteq[0,\infty)=D_{\text{g}}$.
<INSERT\_IMAGE\_HERE>

Hence gf exists.

$[-2,-1)\xrightarrow{f}[\tfrac{1}{3},\infty)\xrightarrow{g}(-\infty,k]$

$R_{\text{gf}}=(-\infty,k]$
\end{enumerate}