\item \textbf{{[}ACJC/PROMO/9758/2021/Q9{]}}
\begin{enumerate}
\item Given that $\sum\limits _{r=1}^{n}r^{2}=\frac{1}{6}n\left(n+1\right)\left(2n+1\right)$,
find $\sum\limits _{r=7}^{n+1}\left(2^{r}+r^{2}-r\right)$ in terms
of $n$. \hfill{}{[}4{]}
\item {}
\begin{enumerate}
\item Use the method of differences to show that $\sum\limits _{r=2}^{n}\frac{1}{r^{2}-1}=\frac{3}{4}+\frac{A}{n}+\frac{A}{n+1}$,
where $A$ is a constant to be determined. \hfill{}{[}3{]}
\item Explain why the series $\sum\limits _{r=2}^{\infty}\frac{1}{r^{2}-1}$
converges, and write down its value. \hfill{}{[}2{]}
\item Hence deduce that $\frac{2}{2^{2}}+\frac{2}{3^{2}}+\frac{2}{4^{2}}+...$
is less than $\frac{3}{2}$. \hfill{}{[}2{]}
\end{enumerate}
\end{enumerate}